Fix and split off ghost stuff for chan spec.

src/goose_lang/lib/channel/chan_spec_multi.v
@@ -1,320 +1,807 @@
-From iris.base_logic.lib Require Import saved_prop.
-From iris.algebra Require Export auth excl frac numbers.
-From iris.base_logic.lib Require Export invariants.
-
 From Perennial.goose_lang Require Import prelude. 
-From Perennial.program_proof.rsm Require Import big_sep.
 From Perennial.goose_lang Require Import notation typing.
 From Perennial.goose_lang Require Import proofmode wpc_proofmode array.
-From Perennial.goose_lang.lib Require Import typed_mem.
-From Perennial.goose_lang Require Export into_val.
+From Perennial.program_proof Require Import proof_prelude.
 From Perennial.program_proof Require Import std_proof.
-From Perennial.goose_lang.lib Require Export
-      persistent_readonly slice slice.typed_slice struct loop lock control map.typed_map time proph rand string.
+From Perennial.goose_lang.automation Require Import extra_tactics.
+From Perennial.goose_lang.lib Require Import
+      persistent_readonly slice slice.typed_slice  struct loop lock control map.typed_map time proph rand string.
 
 From Perennial.goose_lang.lib.channel Require Import auth_set.
+From Perennial.goose_lang.lib.channel Require Import chan_use_ctr.
 From Goose.github_com.goose_lang.goose Require Import channel.
 
-Record chan_names :=
- {
-    sender_name: gname;
-    receiver_name: gname;
-    close_name: gname;
-    close_tok_names_name: gname;
- }.
 
-Class closePropTrackerG Σ := ClosePropTrackerG {
-    sender_main_saved_propG :: savedPropG Σ;
-    close_prop_auth_setG :: auth_setG Σ gname;
-  }.
+Definition in_closed_chan_state (cs: nat): bool :=
+ bool_decide (cs = 5). 
 
-Definition closePropTrackerΣ: gFunctors :=
-  #[ savedPropΣ; auth_setΣ gname ].
-
-#[global] Instance subG_closePropTrackerG Σ : subG closePropTrackerΣ Σ → closePropTrackerG Σ.
-Proof. solve_inG. Qed.
-
-Definition in_closed_state (state: nat): bool :=
- bool_decide (state = 5). 
-
-Inductive chanState: Type := 
+Inductive chan_state: Type := 
 | start
 | receiver_ready
 | sender_ready
 | receiver_done 
 | sender_done
 | closed
+| invalid
 .
 
-Definition nat_to_state (state: nat) : chanState :=
- match state with 
+Section proof.
+Context `{ffi_sem: ffi_semantics} `{!ffi_interp ffi}.
+ Context `{hG: heapGS Σ, !ffi_semantics _ _, !ext_types _}. 
+ Context `{!closePropTrackerG Σ,  !inG Σ (authR (optionUR (prodR fracR natR)))}.
+
+Implicit Types (v:val). 
+
+Definition nat_to_chan_state (cs: nat) : chan_state :=
+ match cs with 
  | 0 => start
  | 1 => receiver_ready
  | 2 => sender_ready
  | 3 => receiver_done
  | 4 => sender_done
  | 5 => closed
- | _ => start
+ | _ => invalid
  end
 .
 
-Section proof.
- Context `{hG: heapGS Σ, !ffi_semantics _ _, !ext_types _}. 
- Context `{!closePropTrackerG Σ,  !inG Σ (authR (optionUR (prodR fracR natR)))}.
-
-Implicit Types (v:val). 
-
-Definition own_chan_counter_frag (γ : gname)
- (n : nat) (q : Qp) : iProp Σ :=
-   own γ (◯ Some (q, n)).
-
-Definition own_chan_counter_auth (γ : gname) 
-   (n : nat) (frozen : bool) : iProp Σ :=
-     own γ (●{if frozen then DfracDiscarded else (DfracOwn 1)} Some (1%Qp, n)).
-
-Definition own_send_counter_frag (γ: chan_names) (n: nat) (q: Qp) : iProp Σ :=
-    own_chan_counter_frag γ.(sender_name) n q.
-
-Definition own_send_counter_auth (γ : chan_names) 
-   (n : nat)  (frozen : bool) : iProp Σ :=
-   own_chan_counter_auth γ.(sender_name) n frozen.
-
-Definition own_recv_counter_frag (γ: chan_names) (n: nat) (q: Qp) : iProp Σ :=
-   own_chan_counter_frag γ.(receiver_name) n q.
-
-Definition own_recv_counter_auth (γ : chan_names) 
-  (n : nat) (frozen : bool) : iProp Σ :=
-  own_chan_counter_auth γ.(receiver_name) n frozen.
-
-Lemma own_chan_counter_split (γ : gname) (n m : nat) (p q : Qp) :
-  own_chan_counter_frag γ (n + m) (p + q) ⊣⊢ own_chan_counter_frag γ n p ∗ own_chan_counter_frag γ m q.
-Proof.
- setoid_rewrite <-own_op.
-  iSplit.
-  { iIntros "H". done. }
-  { iIntros "H". done. }
-Qed.
-
-Lemma own_send_counter_split (γ : chan_names) (n m : nat) (p q : Qp) :
-  own_send_counter_frag γ (n + m) (p + q) ⊣⊢ own_send_counter_frag γ n p ∗ own_send_counter_frag γ m q.
-Proof.
-  unfold own_send_counter_frag. apply own_chan_counter_split.
-Qed.
-
-Lemma own_recv_counter_split (γ : chan_names) (n m : nat) (p q : Qp) :
-  own_recv_counter_frag γ (n + m) (p + q) ⊣⊢ own_recv_counter_frag γ n p ∗ own_recv_counter_frag γ m q.
-Proof.
-  unfold own_recv_counter_frag. apply own_chan_counter_split.
-Qed.
-
-Definition own_closed_tok_frag (γ: chan_names) (γi: gname) (R: iProp Σ): iProp Σ :=
-    auth_set_frag γ.(close_name) γi ∗ saved_prop_own γi (DfracDiscarded) R.
-
-Definition own_closed_tok_auth (γ: chan_names) (R: iProp Σ): iProp Σ :=
-  ∃ (close_tok_names: gset gname),
-    auth_set_auth γ.(close_name) close_tok_names ∗ 
-    (▷R -∗ ([∗ set] γi ∈ close_tok_names,
-                        ∃ Ri, saved_prop_own γi DfracDiscarded Ri ∗  ▷ Ri))                     
-    .
-
-Definition own_closed_tok_post_close (γ: chan_names): iProp Σ := 
-∃ (close_tok_names: gset gname),
-auth_set_auth γ.(close_name) close_tok_names ∗ 
-([∗ set] γi ∈ close_tok_names,
-                    ∃ Ri, saved_prop_own γi DfracDiscarded Ri ∗  ▷ Ri)                  
+Definition chan_state_to_nat (cs: chan_state) : option nat:=
+ match cs with 
+ | start => Some 0
+ | receiver_ready => Some 1
+ | sender_ready => Some 2
+ | receiver_done => Some 3
+ | sender_done => Some 4
+ | closed => Some 5
+ | invalid => None
+ end
 .
 
-Definition own_recv_perm (γ: chan_names) (q: Qp) (i: nat) (T: iProp Σ): iProp Σ :=
- ∃ (γi: gname),
-  own_recv_counter_frag γ i q ∗ own_closed_tok_frag γ γi T .
+Definition is_valid_chan_state (cs: chan_state) : bool :=
+  match cs with
+  | invalid => false
+  | _ => true
+  end.
 
-Definition own_close_perm (γ: chan_names) (R: iProp Σ) (n: nat): iProp Σ :=
-  R ∗ own_send_counter_frag γ n 1 ∗ own_closed_tok_auth γ R.
+Lemma chan_state_eq_dec: ∀ (cs1 cs2: chan_state), {cs1 = cs2} + {cs1 ≠ cs2}.
+Proof.
+  decide equality.
+Qed.
 
-Definition P (q: Qp) (i: nat)
+Lemma chan_state_to_nat_inj: ∀ (cs1 cs2: chan_state),
+  chan_state_to_nat cs1 = chan_state_to_nat cs2 → cs1 = cs2.
+Proof.
+  intros cs1 cs2 H.
+  destruct cs1, cs2; simpl in H; try discriminate; auto.
+Qed.
+
+
+Lemma nts_zero (cs:nat) :
+  cs < 6 -> nat_to_chan_state cs = closed -> cs = 5.
+Proof.
+  intros Hlts. intros Hnts.
+  unfold nat_to_chan_state in Hnts. 
+  do 5(destruct cs;first done). lia.
+Qed.
+
+Definition P (is_single_party: bool) (i:nat)
  (v: val) (Psingle: (nat -> val -> iProp Σ)) (Pmulti: (val -> iProp Σ)): iProp Σ :=
- if bool_decide(q = 1%Qp) then Psingle i v  else Pmulti v.
+ if is_single_party then Psingle i v  else Pmulti v.
 
-Definition Q (q: Qp) (z: Z) (Qsingle: (Z -> iProp Σ)) (Qmulti: iProp Σ): iProp Σ := 
-if bool_decide(Z.lt z 0%Z) then True%I else (if bool_decide(q = 1%Qp) then Qsingle(z) else Qmulti).
-
-
-Lemma own_closed_tok_frag_split (γ : chan_names) (γi: gname) (T U : iProp Σ):
-    ∀ R,
-    (own_closed_tok_auth γ R ∗  own_closed_tok_frag γ γi (T ∗ U) ==∗ 
-    ∃ (γj γk: gname), own_closed_tok_auth γ R ∗ own_closed_tok_frag γ γj T 
-    ∗ own_closed_tok_frag γ γk U
-    ).
-Proof.
-Admitted.
-
-Lemma own_recv_perm_split (γ : chan_names) (r s : Qp) (i k: nat) (T U: iProp Σ) : 
-∀ R,
-own_closed_tok_auth γ R ∗ own_recv_perm γ (r + s) (i + k) (T ∗ U) ==∗   
-own_closed_tok_auth γ R ∗ own_recv_perm γ r i T ∗ own_recv_perm γ s k U.
-Proof.
-Admitted.
+Definition Q (is_single_party: bool) (z: Z) (Qsingle: (Z -> iProp Σ)) (Qmulti: iProp Σ): iProp Σ := 
+if bool_decide(Z.lt z 0%Z) then True%I else (if is_single_party then Qsingle(z) else Qmulti).
 
 Definition isUnbufferedChan (γ: chan_names) (chan_type: ty) 
-  (v: val) (state: nat) (is_single_party: bool) (send_count: nat) (recv_count: nat) (q: Qp) (Psingle: (nat -> val -> iProp Σ)) (Pmulti: (val -> iProp Σ)) (Qsingle: (Z -> iProp Σ)) (Qmulti R: iProp Σ): iProp Σ := 
-    "HStateChanOwns" ∷ 
-     match nat_to_state(state) with 
-      | start => (⌜send_count = recv_count⌝)
-      | receiver_ready => ⌜send_count = recv_count⌝  ∗ Q q recv_count Qsingle Qmulti
-      | sender_ready => ⌜send_count = recv_count ∧ val_ty v chan_type⌝ ∗ P q send_count v Psingle Pmulti 
-      | receiver_done => ⌜recv_count = (send_count + 1)%nat⌝ ∗ Q q recv_count Qsingle Qmulti 
-      | sender_done => ⌜send_count = (recv_count + 1)%nat ∧ val_ty v chan_type⌝ ∗ P q send_count v Psingle Pmulti 
-      | closed => ⌜send_count = recv_count⌝  
+  (v: val) (cs: chan_state) (is_single_party: bool) (send_count: nat) (recv_count: nat) (Psingle: (nat -> val -> iProp Σ)) (Pmulti: (val -> iProp Σ)) (Qsingle: (Z -> iProp Σ)) (Qmulti: iProp Σ )(R:nat ->  iProp Σ): iProp Σ := 
+     match cs with 
+      | start => "%Hcount_eq" ∷ (⌜send_count = recv_count⌝)
+      | receiver_ready => 
+        "%Hcount_eq" ∷ ⌜send_count = recv_count⌝  ∗
+        "HQ" ∷ Q is_single_party recv_count Qsingle Qmulti
+      | sender_ready => 
+        "%Hcount_eq" ∷  ⌜send_count = recv_count⌝ ∗ 
+        "%Hval_ty" ∷  ⌜val_ty v chan_type⌝ ∗ 
+        "HP" ∷  P is_single_party send_count v Psingle Pmulti 
+      | receiver_done => 
+        "%Hcountsendinc" ∷  ⌜recv_count = (send_count + 1)%nat⌝ ∗ 
+        "HQ" ∷ Q is_single_party send_count Qsingle Qmulti 
+      | sender_done => 
+        "%Hcountsendinc" ∷ ⌜send_count = (recv_count + 1)%nat⌝ ∗
+        "HP" ∷   P is_single_party recv_count v Psingle Pmulti ∗
+        "%Hval_ty" ∷  ⌜val_ty v chan_type⌝ 
+      | closed => "%Hcount_eq" ∷ ⌜send_count = recv_count⌝  
+      | invalid => False
      end
   .
 
-  Definition isBufferedChan (γ: chan_names) (chan_type: ty) (size: nat) (state: nat) (is_single_party: bool) (send_count: nat) (recv_count: nat) (count: nat) 
-  (buff: Slice.t) (q: Qp) (Psingle: (nat -> val -> iProp Σ)) (Pmulti: (val -> iProp Σ)) (Qsingle: (Z -> iProp Σ)) (Qmulti R: iProp Σ): iProp Σ := 
+  Definition valid_elems (slice : list val) (first : u64) (count : u64) : list val :=
+  subslice (uint.nat first) (uint.nat first + uint.nat count) (slice ++ slice).
+
+Definition buff_size_inv (count : u64) (first : u64) (size : nat): iProp Σ :=
+  (⌜uint.nat count <= size⌝ ∗ ⌜uint.nat first < size⌝ ∗ ⌜size > 0⌝ ∗ ⌜size + 1 < 2 ^ 63⌝)%I.
+
+  Definition isBufferedChan (γ: chan_names) (chan_type: ty) (size: nat) (cs: chan_state) 
+   (is_single_party: bool) (send_count: nat) (recv_count: nat) (count: nat) 
+  (buff: Slice.t) (first:nat) (Psingle: (nat -> val -> iProp Σ)) (Pmulti: (val -> iProp Σ)) (Qsingle: (Z -> iProp Σ)) (Qmulti: iProp Σ) (R:nat-> iProp Σ): iProp Σ := 
     ∃ (xs: list val), 
-    "%HBuffCount" ∷ ⌜count = (send_count - recv_count)%nat⌝ ∗
+    "%HBuffCount" ∷ ⌜(uint.Z count = (send_count - recv_count)%Z)%Z⌝ ∗
     "HBuffSlice" ∷ slice.own_slice_small buff chan_type (DfracOwn 1) xs ∗ 
-    "%Hcap" ∷ ⌜size = length xs⌝ ∗ 
-    "HPs" ∷ [∗ list] i↦x ∈ xs, (P q (recv_count + i) (nth (recv_count + i) xs (zero_val chan_type)) Psingle Pmulti) ∗ 
-    "HQs" ∷ [∗ list] (i: nat) ∈ (seq 0 (size - send_count + recv_count)), (Q q (recv_count - i + size) Qsingle Qmulti) 
+    "%Hsizeinv" ∷  buff_size_inv count first size ∗ 
+    "%HState" ∷ ⌜cs = start⌝ ∗ 
+    "HPs" ∷ ([∗ list] i↦x ∈ valid_elems xs first count, P is_single_party (recv_count + i) x Psingle Pmulti) ∗ 
+    "HQs" ∷ [∗ list] (i: nat)↦_ ∈ (seqZ 0 (size%Z - send_count%Z + recv_count%Z)), Q is_single_party (recv_count - i + count - 1) Qsingle Qmulti
   .
 
-
-  Definition counters_frozen (state: nat) (send_count: nat) (rec_count: nat): bool :=
-  (in_closed_state state) && bool_decide(send_count = rec_count).
+  Definition counters_frozen (cs: chan_state) (send_count: nat) (rec_count: nat): bool :=
+  match (cs,send_count) with 
+    | (closed,rec_count) => true
+    |  _ => false
+  end
+    .
 
   Definition isChanInner (ch: loc) (γ: chan_names) (chan_type: ty) 
-    (size: nat) (is_single_party: bool) (Psingle: (nat -> val -> iProp Σ)) (Pmulti: (val -> iProp Σ)) (Qsingle: (Z -> iProp Σ)) (Qmulti R: iProp Σ)  : iProp Σ := 
-    ∃ (state: nat) (buff: Slice.t) (count: nat) (first: nat) (v: val) (send_count: nat) (recv_count: nat) (p: dfrac)
-     (q: Qp),
-    "state" ∷ ch ↦[(Channel chan_type) :: "state"] #(W64 state) ∗
+    (size: nat) (is_single_party: bool) (buff: Slice.t) (Psingle: (nat -> val -> iProp Σ)) (Pmulti: (val -> iProp Σ)) (Qsingle: (Z -> iProp Σ)) (Qmulti: iProp Σ) (R: nat -> iProp Σ)  : iProp Σ := 
+    ∃ (raw_cs: nat) (cs: chan_state)  (count: nat) (first: nat) (v: val) (send_count: nat) (recv_count: nat),
+    "chan_state" ∷ ch ↦[(Channel chan_type) :: "state"] #(W64 raw_cs) ∗
     "value" ∷ ch ↦[(Channel chan_type) :: "v"] v ∗ 
     "count" ∷ ch ↦[(Channel chan_type) :: "count"] #(W64 count) ∗ 
     "first" ∷ ch ↦[(Channel chan_type) :: "first"] #(W64 first) ∗ 
-    "#buff" ∷ ch ↦[(Channel chan_type) :: "buff"]□ (slice_val buff) ∗
-    "HSndCtrAuth" ∷ own_send_counter_auth γ send_count (counters_frozen state send_count recv_count) ∗ 
-    "HRcvCtrAuth" ∷ own_recv_counter_auth γ recv_count (counters_frozen state send_count recv_count) ∗ 
-    "HCloseTokPostClose" ∷ if (in_closed_state state) then own_closed_tok_post_close γ
-    else True  ∗ 
-    "%HCounterOwn" ∷ ⌜if is_single_party then q = 1%Qp else (q < 1)%Qp⌝ ∗ 
+    "HSndCtrAuth" ∷ own_send_counter_auth γ send_count (counters_frozen cs send_count recv_count) ∗ 
+    "HRcvCtrAuth" ∷ own_recv_counter_auth γ recv_count (counters_frozen cs send_count recv_count) ∗ 
+    "HCloseTokPostClose" ∷ 
+    match cs with 
+      |closed => (∃ (n:nat), own_closed_tok_post_close γ n ∗  own_send_counter_frag γ n 1 )
+      |_ => True
+     end 
+      ∗ 
+    "%Hvalidstate" ∷ ⌜ chan_state_to_nat cs = Some raw_cs ⌝   ∗  
     "HBuffUnbuff" ∷ 
-    if bool_decide(size = 0) then  
-      isUnbufferedChan γ chan_type v state is_single_party send_count recv_count q Psingle Pmulti
+    match size with 
+      | 0 => isUnbufferedChan γ chan_type v cs is_single_party send_count recv_count  Psingle Pmulti
       Qsingle Qmulti R 
-    else 
-      isBufferedChan γ chan_type size state is_single_party send_count recv_count count
-      buff q Psingle Pmulti Qsingle Qmulti R
+      | S _ => isBufferedChan γ chan_type size cs is_single_party send_count recv_count count
+      buff first Psingle Pmulti Qsingle Qmulti R
+    end 
   .
 
 
 Definition isChan (ch: loc) (γ: chan_names) (chan_type: ty) 
-  (size: nat) (is_single_party: bool) (Psingle: (nat -> val -> iProp Σ)) (Pmulti: (val -> iProp Σ)) (Qsingle: (Z -> iProp Σ)) (Qmulti R: iProp Σ) : iProp Σ := 
-    ∃ (mu_l: loc) ,
+  (size: nat) (is_single_party: bool) (Psingle: (nat -> val -> iProp Σ)) (Pmulti: (val -> iProp Σ)) (Qsingle: (Z -> iProp Σ)) (Qmulti: iProp Σ) (R:nat -> iProp Σ) : iProp Σ := 
+    ∃ (mu_l: loc) (buff: Slice.t) ,
     "#mu" ∷ ch ↦[(Channel chan_type) :: "lock"]□ #mu_l
      ∗ 
-    "#Hlock" ∷ is_lock (nroot .@ "Channel") (#mu_l) (isChanInner ch γ chan_type size is_single_party Psingle Pmulti Qsingle Qmulti R)
+    "#buff" ∷ ch ↦[(Channel chan_type) :: "buffer"]□ (slice_val buff) ∗
+    "#HUnBuffSlice" ∷
+    match size with 
+      | 0 => slice.own_slice_small buff chan_type (DfracDiscarded) []
+      | S _ => True
+    end 
+      ∗ 
+    "#Hlock" ∷ is_lock (nroot .@ "Channel") (#mu_l) (isChanInner ch γ chan_type size is_single_party buff Psingle Pmulti Qsingle Qmulti R)
 .
 
 Lemma wp_Channel__New (γ: chan_names) (chan_type: ty) 
-(size: nat) (is_single_party: bool) (Psingle: (nat -> val -> iProp Σ)) (Pmulti: (val -> iProp Σ)) (Qsingle: (Z -> iProp Σ)) (Qmulti R: iProp Σ) :
+(size: nat) (is_single_party: bool) (Psingle: (nat -> val -> iProp Σ)) (Pmulti: (val -> iProp Σ)) (Qsingle: (Z -> iProp Σ)) (Qmulti: iProp Σ) (R:nat -> iProp Σ) :
+0 < size ∧ size + 1 < 2 ^ 63 ->
+has_zero chan_type ->
 {{{ True }}}
-     NewChannel chan_type #()
+     NewChannelRef chan_type #size
    {{{(ch: loc) (γ: chan_names), RET #ch; 
     isChan ch γ chan_type size is_single_party Psingle Pmulti Qsingle Qmulti R ∗ 
     own_recv_perm γ 1%Qp 0 R ∗
     own_closed_tok_auth γ R ∗ 
     own_send_counter_frag γ 0 1%Qp
 }}}.
-Admitted.
+  Proof.
+    intros Hs Hz.
+  try (iModIntro (□ _)%I);
+  let x := ident:(Φ) in
+  iIntros (Φ) "Hpre HΦ";
+  try wp_rec.
+    rewrite -wp_fupd.
+   wp_apply (wp_new_free_lock). iIntros (mu) "Hlock".
+   wp_pures.
+   wp_apply wp_new_slice;first done.
+   iIntros (slice_ptr) "Hbuffslice".
+   unfold slice.own_slice. 
+  wp_apply(wp_allocStruct (Channel chan_type)).
+  { val_ty. }
+  iIntros (ch). iIntros "Hchan".
+   iNamedStruct "Hchan".
+   iMod (struct_field_pointsto_persist with "lock") as "#mu".
+   iMod (struct_field_pointsto_persist with "buffer") as "#buff".
+   iMod (own_chan_ghost_alloc R) as (γ0) "(HSndAuth & HSndFrag & HRcvAuth & HRcvPrm & HCtf)".
+   destruct size.
+   {
+    iDestruct "Hbuffslice" as "[Hbss Hcap]".
+    iMod ((slice.own_slice_small_persist ) with "Hbss")
+     as "#Hbuffslice". 
+  iMod ((alloc_lock (nroot .@ "Channel") _ mu (
+    (isChanInner ch γ0 chan_type
+    0 is_single_party slice_ptr Psingle Pmulti Qsingle Qmulti R)
+  )) with 
+  "Hlock [ state $v count first HSndAuth HRcvAuth]" ) as "#Hch".
+  {
+    iFrame.
+    iExists 0. iExists start. iExists 0. iExists 0. iExists 0. iExists 0.
+    simpl. unfold counters_frozen. iFrame. done.
+  }
+  {
+    iModIntro. iApply "HΦ". iFrame "#". iFrame. 
+  }
+  }
+  {
+    iMod ((alloc_lock (nroot .@ "Channel") _ mu (
+    (isChanInner ch γ0 chan_type
+    (S size) is_single_party slice_ptr Psingle Pmulti Qsingle Qmulti R)
+  )) with 
+  "Hlock [ state $v count first HSndAuth HRcvAuth Hbuffslice]" ) as "#Hch".
+  {
+    iModIntro. iFrame. iFrame "#". iExists 0. iExists start.
+    iExists 0. iExists 0. iExists 0. iExists 0. unfold counters_frozen.
+    iFrame. simpl. unfold isBufferedChan. simpl. iFrame "#".
+    iSplitL "";first done.
+    iSplitL "";first done. iFrame.
+    iExists ((replicate (uint.nat (W64 (S size)))
+    (zero_val chan_type))). iDestruct "Hbuffslice" as "[H1 H2]".
+    unfold Q. simpl.
+    rewrite -> (big_sepL_forall _ (seqZ 0 (S size - 0%nat + 0%nat))).
+    {
+    iFrame. 
+    do 1 (iSplitL "";first done).
+    unfold buff_size_inv. iFrame "%".
+    simpl. unfold valid_elems.
+    assert ((uint.nat (W64 0%nat) + uint.nat (W64 0%nat)) = 0).
+    { word. }
+    replace ((uint.nat (W64 0%nat) + uint.nat (W64 0%nat))) with 0.
+    assert ((uint.nat (W64 0%nat)) = 0).
+    { done. }
+    replace (uint.nat (W64 0%nat)) with 0. 
+    rewrite subslice_zero_length. simpl. iFrame.
+    do 1 (iSplitL "";first (iPureIntro;lia)).
+    do 2 (iSplitL "";first (iPureIntro;done)).
+    iIntros (k x). iIntros "%Hseq". 
+    rewrite bool_decide_true.
+    { done. }
+    { lia. }
+    }
+    {
+      intros k. intros Z. rewrite bool_decide_true .
+      { 
+        simpl. intuition.
+        unfold Persistent.
+        rewrite persistently_True. done.
+      }
+      {
+        lia.
+      }
+      }
+    }
+      {
+        iModIntro. iApply "HΦ". iFrame "#". iFrame.
+      }
+  }
+  Qed.
 
 Lemma wp_Channel__Send (ch: loc) (i: nat) (v: val) (q: Qp) (γ: chan_names) (chan_type: ty) 
-(size: nat) (is_single_party: bool) (Psingle: (nat -> val -> iProp Σ)) (Pmulti: (val -> iProp Σ)) (Qsingle: (Z -> iProp Σ)) (Qmulti R: iProp Σ) :
+(size: nat) (is_single_party: bool) (Psingle: (nat -> val -> iProp Σ)) (Pmulti: (val -> iProp Σ)) (Qsingle: (Z -> iProp Σ)) (Qmulti: iProp Σ) (R:nat -> iProp Σ) :
 val_ty v chan_type -> 
-(if is_single_party then q = 1%Qp else (q < 1)%Qp) ->
-{{{ isChan ch γ chan_type size is_single_party Psingle Pmulti Qsingle Qmulti R ∗
-  P q i v Psingle Pmulti ∗ own_send_counter_frag γ i q
+#ch ≠ #null ->
+(if is_single_party then q = 1%Qp else ((q < 1)%Qp)) ->
+{{{ 
+  "#HCh" ∷ isChan ch γ chan_type size is_single_party Psingle Pmulti Qsingle Qmulti R ∗
+  "HP" ∷ P is_single_party i v Psingle Pmulti ∗ 
+  "HSen" ∷ own_send_counter_frag γ i q
 }}}
      Channel__Send chan_type #ch v
 {{{ RET #(); 
-  Q q (i - size) Qsingle Qmulti ∗ own_send_counter_frag γ (i + 1)%nat q
+  Q is_single_party (i - size) Qsingle Qmulti ∗ own_send_counter_frag γ (i + 1)%nat q
 }}}.
+  intros Hval_ty. intros Hnotnull. 
+  (* Unbuffered *)
+  destruct (bool_decide (size = 0%nat)) eqn:Hsize.
+  {
+   apply bool_decide_eq_true_1 in Hsize.
+   intros Hq. wp_start. subst size. iNamed "Hpre". iNamed "HCh".
+   wp_if_destruct.
+   {
+    wp_loadField. wp_apply wp_slice_len. 
+    (wp_apply wp_ref_to);first val_ty.
+    iIntros (buf) "Hbuffersize". wp_load.
+     unfold slice.own_slice_small.
+      iDestruct "HUnBuffSlice" as "(#Hbuffsliceptr & %Hbuffsize & %Hcap)".
+      simpl in Hbuffsize.
+      wp_if_destruct;first word.
+      wp_apply wp_ref_to;first val_ty.
+      iIntros (return_early) "return_early".
+        wp_apply (wp_forBreak (λ continue,
+          (
+          "LoopInv_FirstLoop" ∷  ( ∃ (ret_early_b: bool) (send_index: nat), 
+          "LoopInv_RetEarlyFalse" ∷ return_early ↦[boolT] #ret_early_b ∗
+          "LoopInv_SendIndex" ∷  own_send_counter_frag γ send_index q ∗   
+          "LoopInv_Break" ∷  (
+          if continue
+            then 
+            ("%LoopInv_NoRetEarly" ∷ ⌜ret_early_b = false⌝ 
+            ∗ "%LoopInv_SiNoInc" ∷ ⌜send_index = i⌝%I ∗ 
+              "LoopInv_P" ∷ P is_single_party i v Psingle Pmulti)
+          else ( 
+            if ret_early_b then
+              "LoopInv_Q" ∷ Q is_single_party (i) Qsingle Qmulti  ∗ 
+              "%LoopInv_SiInc" ∷ ⌜send_index = (i + 1)%nat⌝%I 
+            else 
+              "%LoopInv_NoRecReady" ∷ ⌜send_index = i%nat⌝ )%I) 
+          ) 
+          ))%I
+          with "[] [HP HSen return_early] [HΦ]").
+          { 
+           iIntros "!>". iIntros (Φ0). iIntros "IH HΦ". iNamed "IH".
+            iNamed "LoopInv_FirstLoop". wp_loadField.
+            wp_apply (wp_Mutex__Lock with "Hlock"). 
+            iIntros "[locked inv]". wp_pures. 
+            iNamed "inv". 
+            unfold isUnbufferedChan. 
+             wp_loadField.
+              destruct cs.
+              {
+                iNamed "LoopInv_Break". iNamed "HBuffUnbuff".
+                simpl in Hvalidstate. assert (raw_cs = 0) by set_solver.
+                wp_pures. subst raw_cs.
+                repeat (wp_loadField||wp_storeField).
+                destruct is_single_party.
+                {
+                  subst q. iDestruct (send_counter_agree with "[$HSndCtrAuth] [$LoopInv_SendIndex]") as "%Hag".
+                  assert (i = send_count) by set_solver.
+                  replace i with send_count.
+                  wp_apply (wp_Mutex__Unlock
+                  with "[$Hlock chan_state value count first HSndCtrAuth HRcvCtrAuth HCloseTokPostClose LoopInv_P $locked]").
+                  { unfold isChanInner. unfold isUnbufferedChan. iModIntro.
+                    iExists 2%nat. iExists sender_ready. iFrame. iPureIntro.
+                    done.
+                  }
+                  {
+                   wp_pures. iModIntro. iApply "HΦ". subst ret_early_b.
+                   iFrame. done. 
+                  }
+                }
+                {
+                  wp_apply (wp_Mutex__Unlock
+                  with "[$Hlock chan_state value count first HSndCtrAuth HRcvCtrAuth HCloseTokPostClose LoopInv_P  $locked]").
+                  { 
+                    unfold isChanInner. unfold isUnbufferedChan. iModIntro.
+                    iExists 2%nat. iExists sender_ready. iFrame. iPureIntro.
+                    done.
+                  }
+                  {
+                    wp_pures. iModIntro. iApply "HΦ". subst ret_early_b.
+                    iFrame. done. 
+                  }
+                }
+              }
+              {
+                iNamed "LoopInv_Break". iNamed "HBuffUnbuff".
+                simpl in Hvalidstate. assert (raw_cs = 1) by set_solver.
+                wp_pures. subst raw_cs.
+                repeat (wp_loadField||wp_storeField).
+                destruct is_single_party.
+                {
+                  subst q. iDestruct (send_counter_agree with "[$HSndCtrAuth] [$LoopInv_SendIndex] ") as "%Heq".
+                  assert (i = send_count) by set_solver.
+                  replace send_count with i.
+                  unfold counters_frozen. unfold in_closed_chan_state. simpl.
+                  iEval (replace i with send_index) in "HSndCtrAuth".
+                  iDestruct ((send_counter_update γ send_index send_index) with "[$HSndCtrAuth $LoopInv_SendIndex]") as ">[HSndCtrAuth LoopInv_SendIndex]".
+                    wp_apply (wp_Mutex__Unlock
+                    with "[ $Hlock $locked chan_state value count first HSndCtrAuth HRcvCtrAuth LoopInv_P ]").
+                    { iModIntro. unfold isChanInner. iExists 4%nat. iExists sender_done.
+                      assert (recv_count = i) by set_solver.
+                      replace recv_count with i by set_solver.
+                      unfold counters_frozen.
+                      iFrame. iPureIntro. unfold chan_state_to_nat. subst send_index.
+                      (do 2 (split;first auto));first lia;val_ty.
+                    } 
+                    { wp_store. iModIntro. iApply "HΦ". iFrame.
+                       replace recv_count with i by set_solver.
+                       iFrame. iPureIntro. lia.
+                    }
+                  }
+                  {
+                    unfold counters_frozen. unfold in_closed_chan_state. simpl.
+                    iDestruct ((send_counter_update γ send_count send_index) with "[$HSndCtrAuth $LoopInv_SendIndex]") as ">[HSndCtrAuth LoopInv_SendIndex]".
+                    wp_apply (wp_Mutex__Unlock
+                    with "[$Hlock $locked chan_state value count first HSndCtrAuth HRcvCtrAuth LoopInv_P]").
+                    { 
+                      iModIntro. unfold isChanInner. iExists 4%nat. iExists sender_done.
+                      iFrame. iPureIntro. 
+                      assert (recv_count = send_count) by set_solver.
+                      replace recv_count with send_count by set_solver.
+                      unfold chan_state_to_nat. 
+                      (do 2 (split;first auto));first lia;val_ty.
+                    }
+                    { 
+                      wp_store. iModIntro. iApply "HΦ". iFrame.
+                      unfold Q. iFrame.
+                      rewrite bool_decide_false.
+                      {
+                        rewrite bool_decide_false. { iFrame. iPureIntro. lia. }
+                        { lia. }
+                      }
+                      destruct recv_count.
+                      { done. }
+                      { done. }
+                    }
+                }
+              }
+              {
+                assert (raw_cs = 2) by set_solver.
+                subst raw_cs.
+                wp_pures.
+                repeat (wp_loadField||wp_storeField).
+                destruct is_single_party.
+                {
+                  subst q. iDestruct (send_counter_agree with "[$HSndCtrAuth] [$LoopInv_SendIndex] ") as "%Hag".
+                  iNamed "HBuffUnbuff".
+                  wp_apply (wp_Mutex__Unlock
+                      with "[$Hlock  $HSndCtrAuth $HRcvCtrAuth $chan_state $value $count $first $locked HP]").
+                      { 
+                        iFrame. done.
+                      }
+                    wp_pures. iModIntro. iApply "HΦ".  iFrame.
+                }
+                {
+                    wp_apply (wp_Mutex__Unlock
+                        with "[$Hlock HBuffUnbuff HSndCtrAuth HRcvCtrAuth chan_state value count first $locked]").
+                        { 
+                            iFrame. done.
+                        }
+                      wp_pures. iModIntro. iApply "HΦ". iFrame.  
+                    } 
+              }
+              {
+                assert (raw_cs = 3) by set_solver.
+                subst raw_cs.
+                wp_pures.
+                repeat (wp_loadField||wp_storeField).
+                wp_apply (wp_Mutex__Unlock
+                    with "[$Hlock HBuffUnbuff HSndCtrAuth HRcvCtrAuth chan_state value count first $locked]").
+                    {
+                      iFrame. done.
+                    }
+                  wp_pures. iModIntro. iApply "HΦ". iFrame. 
+                }
+                {
+                assert (raw_cs = 4) by set_solver.
+                subst raw_cs.
+                wp_pures.
+                repeat (wp_loadField||wp_storeField).
+                wp_apply (wp_Mutex__Unlock
+                    with "[$Hlock HBuffUnbuff HSndCtrAuth HRcvCtrAuth chan_state value count first $locked]").
+                    { 
+                      iFrame. done.
+                    }
+                  wp_pures. iModIntro. iApply "HΦ". iFrame.  
+                }
+                {
+                  assert (raw_cs = 5) by set_solver.
+                subst raw_cs.
+                wp_pures. iNamed "HCloseTokPostClose". iDestruct "HCloseTokPostClose" as "[Hct Hsc]".
+                iCombine "Hsc" "LoopInv_SendIndex" as "H" gives %Hvalid. 
+                  apply auth_frag_op_valid_1 in Hvalid.
+                  rewrite <- (Some_op (1%Qp, x) (q, send_index)) in Hvalid.
+                  rewrite Some_valid in Hvalid.
+                  rewrite <- (pair_op 1%Qp q x send_index) in Hvalid.
+                  rewrite pair_valid in Hvalid. destruct Hvalid as [Hqvalid Hivalid].
+                  rewrite frac_op in Hqvalid.
+                  assert (((1 + q)%Qp ≤ 1)%Qp).
+                  { done. }
+                  apply Qp.not_add_le_l in H.
+                  contradiction.
+                }
+                {
+                 done. 
+                }
+          }
+          {
+            iFrame. done.
+          }
+          {
+            iModIntro. iIntros "IH". iNamed "IH". 
+            iNamed "LoopInv_FirstLoop".
+            wp_pures.  
+            destruct ret_early_b.
+            {
+              wp_load. wp_pures.
+              wp_apply (wp_forBreak (λ continue,
+              (
+                "LoopInv_Wrapper" ∷  ( ∃ (ret_early_b: bool) (send_index: nat), 
+                "LoopInv_SendIndex" ∷  (own_send_counter_frag γ send_index q) ∗   
+                "HQ" ∷ Q is_single_party (i) Qsingle Qmulti ∗
+                "%LoopInv_SiInc" ∷ ⌜send_index = (i + 1)%nat⌝
+              )))%I
+              with "[] [LoopInv_RetEarlyFalse LoopInv_SendIndex LoopInv_Break] [HΦ]").
+              {    
+                  iIntros "!>" (Φ0) "IH HΦ". iNamed "IH". iNamed "LoopInv_Wrapper".
+                  wp_loadField.
+                  wp_apply (wp_Mutex__Lock with "Hlock"). 
+                  iIntros "[locked inv]". wp_pures.
+                  iNamed "inv". wp_loadField.
+                  wp_if_destruct.
+                  {
+                    wp_loadField.
+                    wp_apply (wp_Mutex__Unlock
+                    with "[$Hlock HBuffUnbuff HCloseTokPostClose HSndCtrAuth HRcvCtrAuth chan_state value count first $locked]").
+                    { 
+                     iFrame. done.
+                    } 
+                    {
+                      wp_pures. iModIntro. iApply "HΦ". iFrame. done.  
+                    }
+                  }
+                  {
+                    wp_pures. 
+                      wp_loadField.
+                      assert (raw_cs = 4).
+                      { 
+                        unfold chan_state_to_nat in Hvalidstate.
+                        destruct cs; do 7 (set_solver).
+                      }
+                      subst raw_cs.
+                        wp_apply (wp_Mutex__Unlock
+                        with "[$Hlock HBuffUnbuff HSndCtrAuth HRcvCtrAuth chan_state value count first $locked]").
+                        { 
+                          iFrame "%#". iFrame. unfold chan_state_to_nat in Hvalidstate.
+                          assert (cs = sender_done).
+                          { destruct cs; do 6 (done). }
+                          subst cs. done.
+                        }
+                        {
+                         wp_pures. iModIntro. iApply "HΦ". iFrame. done. 
+                        }
+                     } 
+                    } 
+                    { 
+                      iFrame. done.
+                    }
+                    {
+                      iModIntro. iIntros "IH". iNamed "IH". iNamed "LoopInv_Wrapper".
+                      wp_pures. iModIntro. iApply "HΦ". iNamed "HQ". subst send_index0.
+                      iFrame. unfold Q. 
+                      destruct i.
+                      { simpl. done. }
+                      simpl. done.
+                    }
+            }
+            {
+              wp_load. wp_pures.  iNamed "LoopInv_Break".
+              wp_apply (wp_forBreak (λ continue,
+                (
+                "LoopInv_LastLoop" ∷  ( ∃ (ret_early_b: bool) (send_index: nat), 
+                "LoopInv_SendIndex" ∷  (own_send_counter_frag γ send_index q) ∗   
+                "%LoopInv_Break" ∷  (if continue
+                then ("%LoopInv_Cont" ∷ ⌜(send_index = i)⌝%I)
+                else ("HQ" ∷ Q is_single_party (i) Qsingle Qmulti  ∗ "%LoopInv_SiInc" ∷ ⌜send_index = (i + 1)%nat⌝ )%I) 
+                ) 
+                ))%I
+                with "[] [LoopInv_SendIndex] [HΦ]").
+                { 
+                  iIntros "!>". iIntros (Φ0). iIntros "IH HΦ". iNamed "IH".
+                  iNamed "LoopInv_LastLoop". wp_loadField.
+                  wp_apply (wp_Mutex__Lock with "Hlock"). 
+                  iIntros "[locked inv]". wp_pures.
+                  iNamed "inv".  iNamed "HBuffUnbuff".
+                  unfold isUnbufferedChan. iNamed "HBuffUnbuff". wp_loadField.
+                  wp_if_destruct.
+                  {
+                   assert (raw_cs = 5).
+                   { 
+                    unfold chan_state_to_nat in Hvalidstate.
+                    do 1 (destruct cs;do 5 (set_solver)). 
+                   } 
+                   subst raw_cs. assert (cs = closed).
+                   { destruct cs;do 5 (set_solver). }
+                   subst cs.
+                    wp_pures. iNamed "HCloseTokPostClose". iDestruct "HCloseTokPostClose" as "[Hct Hsc]".
+                    iCombine "Hsc" "LoopInv_SendIndex" as "H" gives %Hvalid. 
+                      apply auth_frag_op_valid_1 in Hvalid.
+                      rewrite <- (Some_op (1%Qp, n) (q, i)) in Hvalid.
+                      rewrite Some_valid in Hvalid.
+                      rewrite <- (pair_op 1%Qp q n i) in Hvalid.
+                      rewrite pair_valid in Hvalid. destruct Hvalid as [Hqvalid Hivalid].
+                      rewrite frac_op in Hqvalid.
+                      assert (((1 + q)%Qp ≤ 1)%Qp).
+                      { done. }
+                      apply Qp.not_add_le_l in Hqvalid.
+                      contradiction.
+                   }
+                   {
+                    wp_pures. 
+                     wp_pures. wp_loadField. 
+                     wp_if_destruct.
+                     {
+                        wp_storeField. wp_loadField.
+                        assert (raw_cs = 3%nat).
+                        { destruct cs;do 7 (set_solver). }
+                        assert (cs = receiver_done).
+                        { destruct cs; do 7 (set_solver). }
+                        subst cs.
+                        iNamed "HBuffUnbuff".
+                        iDestruct ((send_counter_update γ send_count i) with "[HSndCtrAuth LoopInv_SendIndex]") as ">HFupdStuff".
+                        { iFrame. }
+                        iDestruct "HFupdStuff" as "[HSndCtrAuth LoopInv_SendIndex]". 
+                        destruct is_single_party.
+                          {
+                            subst q. iDestruct (send_counter_agree with "[$HSndCtrAuth] [$LoopInv_SendIndex] ") as "%Hag".
+                            subst recv_count.
+                              wp_apply (wp_Mutex__Unlock
+                              with "[$Hlock chan_state $value $count $first $locked HSndCtrAuth HRcvCtrAuth ]").
+                              {
+                                iModIntro.
+                                unfold isChanInner. iExists 0%nat. iExists start.
+                                 iFrame. unfold counters_frozen.
+                                iFrame "%#".
+                                iFrame. simpl. iPureIntro.
+                                do 2 split;first done.
+                                lia.
+                              }
+                              {
+                                wp_pures. iModIntro. iApply "HΦ". iFrame. 
+                                
+                                unfold Q. rewrite bool_decide_false.
+                                {
+                                  rewrite bool_decide_false.
+                                  {
+                                    assert (send_count = i).
+                                    { lia. }
+                                    subst send_count. destruct i.
+                                    { iFrame. done. }
+                                    iFrame. iPureIntro. exists.
+                                    { done. }
+                                    lia.
+                                  } { lia. }
+                                } lia. 
+                              }
+                          }
+                          {
+                            subst recv_count.
+                            wp_apply (wp_Mutex__Unlock
+                              with "[$Hlock chan_state $value $count $first HSndCtrAuth HRcvCtrAuth 
+                              $locked]").
+                              {
+                                iModIntro. iExists 0. iExists start. iFrame. 
+                                unfold counters_frozen. simpl. iFrame.
+                                iPureIntro.
+                                do 2 split;first done.
+                                lia.
+                              }
+                              {
+                          
+                                wp_pures. iModIntro. iApply "HΦ". iFrame. 
+                                unfold Q. 
+                                rewrite bool_decide_false.
+                                {
+                                destruct i. { iFrame. done. }
+                                 { 
+                                  iFrame. iPureIntro. exists. { done. }
+                                  lia.
+                                 } 
+                                } lia.
+                              }
+                          }
+                    }
+                    {
+                      wp_loadField.
+                      wp_apply (wp_Mutex__Unlock
+                              with "[$Hlock HSndCtrAuth HRcvCtrAuth chan_state value count first 
+                              HBuffUnbuff HCloseTokPostClose $locked]").
+                              {
+                                iFrame. done.
+                              }
+                              
+                              {
+                                wp_pures. iModIntro. iApply "HΦ". iFrame. done.
+                              }
+                    }
+                  }
+              }
+            {
+              iFrame. done.
+            }
+            {
+              iModIntro. iIntros "IH". iNamed "IH". wp_pures. iApply "HΦ".
+              iModIntro. iNamed "LoopInv_LastLoop". iFrame. subst send_index0.
+              iFrame. destruct i.
+              {
+                done.
+              }
+              done.
+            }
+          }
+        }
+      }
+     }
+  {
+    (* buffered channels *)
+    admit.
+  }
 Admitted.
 
 Lemma wp_Channel__TrySend (ch: loc) (i: nat) (v: val) (q: Qp) (γ: chan_names) (chan_type: ty) 
-(size: nat) (is_single_party: bool) (Psingle: (nat -> val -> iProp Σ)) (Pmulti: (val -> iProp Σ)) (Qsingle: (Z -> iProp Σ)) (Qmulti R: iProp Σ) :
+(size: nat) (is_single_party: bool) (Psingle: (nat -> val -> iProp Σ)) (Pmulti: (val -> iProp Σ)) (Qsingle: (Z -> iProp Σ)) (Qmulti: iProp Σ) (R:nat -> iProp Σ) :
 val_ty v chan_type -> 
+#ch ≠ #null ->
 (if is_single_party then q = 1%Qp else (q < 1)%Qp) ->
 {{{ isChan ch γ chan_type size is_single_party Psingle Pmulti Qsingle Qmulti R ∗
-  P q i v Psingle Pmulti ∗ own_send_counter_frag γ i q
+  P is_single_party i v Psingle Pmulti ∗ own_send_counter_frag γ i q
 }}}
      Channel__TrySend chan_type #ch v
 {{{ (selected: bool), RET #selected; 
   if selected then 
-    (Q q (i - size) Qsingle Qmulti ∗ own_send_counter_frag γ (i + 1)%nat q)
+    (Q is_single_party (i - size) Qsingle Qmulti ∗ own_send_counter_frag γ (i + 1)%nat q)
   else 
-    ( P q i v Psingle Pmulti ∗ own_send_counter_frag γ i q) 
+    ( P is_single_party i v Psingle Pmulti ∗ own_send_counter_frag γ i q) 
 }}}.
 Admitted.
 
 Lemma wp_Channel__Receive (ch: loc) (i: nat) (q: Qp) (γ: chan_names) (chan_type: ty) 
-(size: nat) (is_single_party: bool) (Psingle: (nat -> val -> iProp Σ)) (Pmulti: (val -> iProp Σ)) (Qsingle: (Z -> iProp Σ)) (Qmulti R: iProp Σ) :
+(size: nat) (is_single_party: bool) (Psingle: (nat -> val -> iProp Σ)) (Pmulti: (val -> iProp Σ)) (Qsingle: (Z -> iProp Σ)) (Qmulti: iProp Σ) (R:nat -> iProp Σ) :
+#ch ≠ #null ->
 (if is_single_party then q = 1%Qp else (q < 1)%Qp) ->
-∃ (Ri: iProp Σ),
+∃ (Ri:nat -> iProp Σ),
 {{{ 
   isChan ch γ chan_type size is_single_party Psingle Pmulti Qsingle Qmulti R ∗
-  Q q i Qsingle Qmulti ∗ 
+  Q is_single_party i Qsingle Qmulti ∗ 
   own_recv_perm γ q i Ri 
 }}}
      Channel__Receive chan_type #ch
 {{{ (v: val) (ok: bool), RET (v,#ok); 
-  (P q i v Psingle Pmulti ∗ own_recv_perm γ q (i + 1) Ri ∗ ⌜ok⌝ ∗ ⌜val_ty v chan_type⌝)
+  (P is_single_party i v Psingle Pmulti ∗ own_recv_perm γ q (i + 1) Ri ∗ ⌜ok⌝ ∗ ⌜val_ty v chan_type⌝)
     ∨  
-  (Ri ∗ own_recv_counter_frag γ i q ∗ ⌜v = (zero_val chan_type)⌝ ∗ ⌜ok = false⌝
-    ∗ ∃ n, own_send_counter_auth γ n true ∗ own_recv_counter_auth γ n true)
+  ( own_recv_counter_frag γ i q ∗ ⌜v = (zero_val chan_type)⌝ ∗ ⌜ok = false⌝
+    ∗ ∃ n, (Ri n) ∗ own_send_counter_auth γ n true ∗ own_recv_counter_auth γ n true)
 }}}.
 Admitted.
 
 Lemma wp_Channel__ReceiveDiscardOk (ch: loc) (i: nat) (q: Qp) (γ: chan_names) (chan_type: ty) 
-(size: nat) (is_single_party: bool) (Psingle: (nat -> val -> iProp Σ)) (Pmulti: (val -> iProp Σ)) (Qsingle: (Z -> iProp Σ)) (Qmulti R: iProp Σ) :
+(size: nat) (is_single_party: bool) (Psingle: (nat -> val -> iProp Σ)) (Pmulti: (val -> iProp Σ)) (Qsingle: (Z -> iProp Σ)) (Qmulti: iProp Σ) (R:nat -> iProp Σ) :
+#ch ≠ #null ->
 (if is_single_party then q = 1%Qp else (q < 1)%Qp) ->
-∃ (Ri: iProp Σ),
+∃ (Ri:nat -> iProp Σ),
 {{{ 
   isChan ch γ chan_type size is_single_party Psingle Pmulti Qsingle Qmulti R ∗
-  Q q i Qsingle Qmulti ∗ 
+  Q is_single_party i Qsingle Qmulti ∗ 
   own_recv_perm γ q i Ri 
 }}}
      Channel__ReceiveDiscardOk chan_type #ch
 {{{ (v: val), RET (v); 
-  (P q i v Psingle Pmulti ∗ own_recv_perm γ q (i + 1) Ri ∗ ⌜val_ty v chan_type⌝)
+  (P is_single_party i v Psingle Pmulti ∗ own_recv_perm γ q (i + 1) Ri ∗ ⌜val_ty v chan_type⌝)
     ∨  
-  (Ri ∗ own_recv_counter_frag γ i q ∗ ⌜v = (zero_val chan_type)⌝
-    ∗ ∃ n, own_send_counter_auth γ n true ∗ own_recv_counter_auth γ n true)
+  (own_recv_counter_frag γ i q ∗ ⌜v = (zero_val chan_type)⌝
+    ∗ ∃ n, (Ri n) ∗ own_send_counter_auth γ n true ∗ own_recv_counter_auth γ n true)
 }}}.
 Admitted.
 
 Lemma wp_Channel__TryReceive (ch: loc) (i: nat) (q: Qp) (γ: chan_names) (chan_type: ty) 
-(size: nat) (is_single_party: bool) (Psingle: (nat -> val -> iProp Σ)) (Pmulti: (val -> iProp Σ)) (Qsingle: (Z -> iProp Σ)) (Qmulti R: iProp Σ) :
+(size: nat) (is_single_party: bool) (Psingle: (nat -> val -> iProp Σ)) (Pmulti: (val -> iProp Σ)) (Qsingle: (Z -> iProp Σ)) (Qmulti: iProp Σ) (R:nat -> iProp Σ) :
 (if is_single_party then q = 1%Qp else (q < 1)%Qp) ->
-∃ (Ri: iProp Σ),
+∃ (Ri:nat -> iProp Σ),
 {{{ 
   isChan ch γ chan_type size is_single_party Psingle Pmulti Qsingle Qmulti R ∗
-  Q q i Qsingle Qmulti ∗ own_recv_perm γ q i Ri 
+  Q is_single_party i Qsingle Qmulti ∗ own_recv_perm γ q i Ri 
 }}}
      Channel__TryReceive chan_type #ch
 {{{ (v: val) (ok: bool) (selected: bool), RET (#selected,v,#ok); 
   if selected then 
-    ((P q i v Psingle Pmulti ∗ own_recv_perm γ q (i + 1) Ri ∗ ⌜ok⌝ ∗ ⌜val_ty v chan_type⌝)
+    ((P is_single_party i v Psingle Pmulti ∗ own_recv_perm γ q (i + 1) Ri ∗ ⌜ok⌝ ∗ ⌜val_ty v chan_type⌝)
     ∨  
-    (Ri ∗ own_recv_counter_frag γ i q ∗ ⌜v = (zero_val chan_type)⌝ ∗ ⌜ok = false⌝
-      ∗ ∃ n, own_send_counter_auth γ n true ∗ own_recv_counter_auth γ n true)
+    ( own_recv_counter_frag γ i q ∗ ⌜v = (zero_val chan_type)⌝ ∗ ⌜ok = false⌝
+      ∗ ∃ n, (Ri n) ∗ own_send_counter_auth γ n true ∗ own_recv_counter_auth γ n true)
     )
   else 
-    ( Q q i Qsingle Qmulti ∗ own_recv_perm γ q i Ri)
+    ( Q is_single_party i Qsingle Qmulti ∗ own_recv_perm γ q i Ri)
 }}}.
 Admitted.
 
 Lemma wp_Channel__Close (ch: loc) (n: nat) (γ: chan_names) (chan_type: ty) 
-(size: nat) (is_single_party: bool) (Psingle: (nat -> val -> iProp Σ)) (Pmulti: (val -> iProp Σ)) (Qsingle: (Z -> iProp Σ)) (Qmulti R: iProp Σ) :
-∃ (Ri: iProp Σ),
+(size: nat) (is_single_party: bool) (Psingle: (nat -> val -> iProp Σ)) (Pmulti: (val -> iProp Σ)) (Qsingle: (Z -> iProp Σ)) (Qmulti: iProp Σ) (R:nat -> iProp Σ) :
 {{{ 
   isChan ch γ chan_type size is_single_party Psingle Pmulti Qsingle Qmulti R ∗
   own_close_perm γ R n
